Updated union-judgements and super/subtype-judgements

books/projects/smtlink/verified/type-inference.lisp
@@ -30,24 +30,13 @@
 
 ;; Datatypes and functions that operates them
 
-;; This is a version where a type can have multiple supertypes
-;; (defalist type-to-supertypes-alist
-;;   :key-type symbolp
-;;   :val-type symbol-listp
-;;   :true-listp t)
-
-;; (defthm assoc-equal-of-type-to-supertypes-alist
-;;   (implies (and (type-to-supertypes-alist-p x)
-;;                 (assoc-equal y x))
-;;            (consp (assoc-equal y x))))
-
-(defalist type-to-type-alist
+(defalist type-to-types-alist
   :key-type symbolp
-  :val-type symbolp
+  :val-type symbol-listp
   :true-listp t)
 
-(defthm assoc-equal-of-type-to-type-alist
-  (implies (and (type-to-type-alist-p x)
+(defthm assoc-equal-of-type-to-types-alist
+  (implies (and (type-to-types-alist-p x)
                 (assoc-equal y x))
            (consp (assoc-equal y x))))
 
@@ -59,6 +48,12 @@
   :key-type type-tuple-p
   :val-type symbolp
   :true-listp t)
+
+(defthm assoc-equal-of-type-tuple-to-thm-alist
+  (implies (and (type-tuple-to-thm-alist-p x)
+                (assoc-equal y x))
+           (and (consp (assoc-equal y x))
+                (symbolp (cdr (assoc-equal y x))))))
 
 (defprod return-spec
   ((return-type symbolp)
@@ -169,8 +164,7 @@
    (some-type symbolp)
    (some-constructor-thm symbolp)
    (none-constructor-thm symbolp)
-   (some-destructor-thm symbolp)
-   (non-nil-thm symbolp)))
+   (some-destructor-thm symbolp)))
 
 (defalist option-type-description-alist
   :key-type symbolp
@@ -195,9 +189,9 @@
   :true-listp t)
 
 (defprod type-options
-  ((supertype type-to-type-alist-p)
+  ((supertype type-to-types-alist-p)
    (supertype-thm type-tuple-to-thm-alist-p)
-   (subtype type-to-type-alist-p)
+   (subtype type-to-types-alist-p)
    (subtype-thm type-tuple-to-thm-alist-p)
    (functions function-description-alist-p)
    (consp cons-type-description-alist-p)
@@ -210,26 +204,10 @@
    (abstract abstract-type-description-alist-p)))
 )
 
-(define is-maybe-type? ((type symbolp)
-                        (option option-type-description-alist-p))
-  :returns (ok booleanp)
-  (not (null (assoc-equal type (option-type-description-alist-fix option)))))
-
-(define get-nonnil-thm ((type symbolp)
-                        (option option-type-description-alist-p))
-  :returns (thm symbolp)
-  (b* ((option (option-type-description-alist-fix option))
-       (conspair (assoc-equal type option))
-       ((unless conspair)
-        (er hard? 'type-inference=>get-nonnil-thm
-            "Can't find type ~p0 in the option-type alist.~%" type))
-       (type-description (cdr conspair)))
-    (option-type-description->non-nil-thm type-description)))
-
 (define is-type? ((type symbolp)
-                  (supertype-alst type-to-type-alist-p))
+                  (supertype-alst type-to-types-alist-p))
   :returns (ok booleanp)
-  (not (null (assoc-equal type (type-to-type-alist-fix supertype-alst)))))
+  (not (null (assoc-equal type (type-to-types-alist-fix supertype-alst)))))
 
 ;; ------------------------
 
@@ -254,7 +232,7 @@
   (only-one-var-acc term-lst term 0))
 
 (define type-predicate-p ((judge pseudo-termp)
-                          (supertype-alst type-to-type-alist-p))
+                          (supertype-alst type-to-types-alist-p))
   :returns (ok booleanp)
   (and (pseudo-termp judge)
        (equal (len judge) 2)
@@ -271,7 +249,7 @@
 
 (define type-predicate-of-term ((judge pseudo-termp)
                                 (term pseudo-termp)
-                                (supertype-alst type-to-type-alist-p))
+                                (supertype-alst type-to-types-alist-p))
   :returns (ok booleanp)
   (and (pseudo-termp judge)
        (equal (len judge) 2)
@@ -291,7 +269,7 @@
 
 (define judgement-of-term ((judge pseudo-termp)
                            (term pseudo-termp)
-                           (supertype-alst type-to-type-alist-p))
+                           (supertype-alst type-to-types-alist-p))
   :returns (ok booleanp)
   (or (equal judge term)
       (type-predicate-of-term judge term supertype-alst)
@@ -426,7 +404,7 @@
 ;; level and's
 (define look-up-path-cond-acc ((term pseudo-termp)
                                (path-cond pseudo-termp)
-                               (supertype-alst type-to-type-alist-p)
+                               (supertype-alst type-to-types-alist-p)
                                (acc pseudo-termp))
   :returns (type-term pseudo-termp)
   :measure (acl2-count (pseudo-term-fix path-cond))
@@ -446,7 +424,7 @@
 
 (define look-up-path-cond ((term pseudo-termp)
                            (path-cond pseudo-termp)
-                           (supertype-alst type-to-type-alist-p))
+                           (supertype-alst type-to-types-alist-p))
   :returns (type-term pseudo-termp)
   (look-up-path-cond-acc term path-cond supertype-alst ''t))
 
@@ -579,373 +557,47 @@
             "The top of type judgement is not a conjunction of conditions: ~q0"
             judgements-lst))
        ((if (equal judgements-lst ''t)) ''t)
-       ((list* & judgements-hd judgements-tl &) judgements-lst))
+       ((list & judgements-hd judgements-tl &) judgements-lst))
     `(if ,(type-judgement-top judgements-hd)
          ,(type-judgement-top-list judgements-tl)
        'nil)))
 
-;;-----------------------
-;;      subtyping
+;;-------------------------------------------------------
 
-;; (defines supertype-transitive-closure
-;;   :well-founded-relation l<
-;;   :verify-guards nil
-
-;;   (define supertype ((type symbolp)
-;;                      (supertype-alst
-;;                       type-to-supertypes-alist-p)
-;;                      (closure symbol-listp)
-;;                      (clock natp)) ;; clock is the length of the supertype-alst
-;;     :measure (list (nfix clock) (acl2-count (symbol-fix type)))
-;;     :returns (closure symbol-listp)
-;;     (b* ((type (symbol-fix type))
-;;          (supertype-alst (type-to-supertypes-alist-fix supertype-alst))
-;;          (closure (symbol-list-fix closure))
-;;          (clock (nfix clock))
-;;          ((if (zp clock)) closure)
-;;          (exist? (member-equal type closure))
-;;          ((if exist?) closure)
-;;          (new-closure (cons type closure))
-;;          (item (assoc-equal type supertype-alst))
-;;          ((unless item)
-;;           (er hard? 'type-inference=>supertype
-;;               "Type ~p0 doesn't exist in the supertype alist.~%" type))
-;;          ((unless (cdr item)) new-closure)
-;;          (supertype-lst (cdr item)))
-;;       (supertype-list supertype-lst supertype-alst new-closure (1- clock))))
-
-;;   (define supertype-list ((type-lst symbol-listp)
-;;                           (supertype-alst
-;;                            type-to-supertypes-alist-p)
-;;                           (closure symbol-listp)
-;;                           (clock natp))
-;;     :measure (list (nfix clock) (acl2-count (symbol-list-fix type-lst)))
-;;     :returns (closure symbol-listp)
-;;     (b* ((type-lst (symbol-list-fix type-lst))
-;;          (supertype-alst (type-to-supertypes-alist-fix supertype-alst))
-;;          (closure (symbol-list-fix closure))
-;;          (clock (nfix clock))
-;;          ((unless (consp type-lst)) closure)
-;;          ((cons type-hd type-tl) type-lst)
-;;          (new-closure
-;;           (supertype type-hd supertype-alst closure clock)))
-;;       (supertype-list type-tl supertype-alst new-closure clock)))
-;;   )
-;;
-;; (verify-guards supertype)
-
-(defthm symbolp-of-cdr-of-assoc-equal-from-type-to-type-alist
-  (implies (and (type-to-type-alist-p x)
-                (assoc-equal y x))
-           (symbolp (cdr (assoc-equal y x)))))
-
-(define supertype-clocked ((type symbolp)
-                           (supertype-alst type-to-type-alist-p)
-                           (clock natp))
-  :returns (supertypes symbol-listp)
-  :measure (nfix clock)
-  (b* ((type (symbol-fix type))
-       (supertype-alst (type-to-type-alist-fix supertype-alst))
-       (clock (nfix clock))
-       ((if (zp clock))
-        (er hard? 'type-inference=>supertype
-            "Run out of clocks.~%"))
-       (conspair (assoc-equal type supertype-alst))
-       ((unless (and conspair (cdr conspair))) nil))
-    (cons (cdr conspair)
-          (supertype-clocked (cdr conspair) supertype-alst (1- clock)))))
-
-;; -----------------------------------------------------
-
-(define look-up-type-tuple-to-thm-alist ((root-type symbolp)
-                                         (super-type symbolp)
-                                         (thms type-tuple-to-thm-alist-p)
-                                         state)
-  :returns (ok booleanp)
-  :ignore-ok t
-  (b* ((thms (type-tuple-to-thm-alist-fix thms))
-       (tuple (make-type-tuple :type root-type
-                               :neighbour-type super-type))
-       (conspair (assoc-equal tuple thms))
-       ((unless conspair)
-        (er hard? 'type-inference=>supertype-to-judgements
-            "There doesn't exist a theorem supporting the supertype ~
-             relationship between ~p0 and ~p1.~%"
-            root-type super-type))
-       (thm-name (cdr conspair))
-       (supertype-thm
-        (acl2::meta-extract-formula-w thm-name (w state)))
-       ((unless (pseudo-termp supertype-thm))
-        (er hard? 'type-inference=>supertype-to-judgements
-            "Formula returned by meta-extract ~p0 is not a pseudo-termp: ~p1~%"
-            thm-name supertype-thm))
-       (ok (case-match supertype-thm
-             (('implies (!root-type var)
-                        (!super-type var)) t)
-             (& nil)))
-       ((unless ok)
-        (er hard? 'type-inference=>supertype-to-judgements
-            "Type: ~p0, supertype: ~p1, supertype theorem is malformed: ~p2~%"
-            root-type super-type supertype-thm)))
-    t))
-
-
-(encapsulate ()
-  (local (in-theory (disable (:definition pseudo-termp)
-                             (:rewrite lambda-of-pseudo-lambdap))))
-  (local
-   (defthm assoc-equal-of-type-tuple-to-thm-alist-p
-     (implies (and (type-tuple-to-thm-alist-p x)
-                   (assoc-equal y x))
-              (and (consp (assoc-equal y x))
-                   (symbolp (cdr (assoc-equal y x)))))))
-
-(define supertype-to-judgements ((root-type symbolp)
-                                 (supertypes symbol-listp)
-                                 (term pseudo-termp)
-                                 (thms type-tuple-to-thm-alist-p)
-                                 (acc pseudo-termp)
-                                 state)
-  :returns (judgements pseudo-termp)
-  :measure (len supertypes)
-  (b* ((root-type (symbol-fix root-type))
-       (supertypes (symbol-list-fix supertypes))
-       (term (pseudo-term-fix term))
-       (thms (type-tuple-to-thm-alist-fix thms))
-       (acc (pseudo-term-fix acc))
-       ((unless (consp supertypes)) acc)
-       ((cons supertypes-hd supertypes-tl) supertypes)
-       ((unless
-            (look-up-type-tuple-to-thm-alist root-type supertypes-hd thms state))
-        nil)
-       (supertype-term `(,supertypes-hd ,term))
-       ((if (path-test acc supertype-term state))
-        (supertype-to-judgements root-type supertypes-tl term thms acc state)))
-    (supertype-to-judgements root-type supertypes-tl term thms
-                             `(if ,supertype-term ,acc 'nil) state)))
-)
-
-(define supertype-judgement-single ((type-judgement pseudo-termp)
-                                    (supertype-alst type-to-type-alist-p)
-                                    (thms type-tuple-to-thm-alist-p)
-                                    (acc pseudo-termp)
-                                    state)
-  :returns (judgements pseudo-termp)
-  (b* ((type-judgement (pseudo-term-fix type-judgement))
-       (acc (pseudo-term-fix acc))
-       ((unless (type-predicate-p type-judgement supertype-alst))
-        (er hard? 'type-inference=>supertype-judgement-single
-            "Type judgement ~p0 is malformed.~%" type-judgement))
-       ((list root-type term) type-judgement)
-       (supertype-alst (type-to-type-alist-fix supertype-alst))
-       (clock (len supertype-alst))
-       (supertypes
-        (supertype-clocked root-type supertype-alst clock)))
-    (supertype-to-judgements root-type supertypes term thms acc state)))
-
-(define supertype-judgements-acc ((judge pseudo-termp)
-                                  (supertype-alst type-to-type-alist-p)
-                                  (thms type-tuple-to-thm-alist-p)
-                                  (acc pseudo-termp)
-                                  state)
-  :returns (judgements pseudo-termp)
-  :measure (acl2-count (pseudo-term-fix judge))
-  (b* ((judge (pseudo-term-fix judge))
-       (acc (pseudo-term-fix acc))
-       ((unless (is-conjunct? judge))
-        (er hard? 'type-inference=>supertype-judgements
-            "~p0 is not a conjunction.~%" judge))
-       ((if (equal judge ''t)) acc)
-       ((list* & cond then &) judge)
-       (first-acc
-        (supertype-judgement-single cond supertype-alst thms acc state)))
-    (supertype-judgements-acc then supertype-alst thms first-acc state)))
-
-(define supertype-judgements ((judge pseudo-termp)
-                              (supertype-alst type-to-type-alist-p)
-                              (thms type-tuple-to-thm-alist-p)
+(define union-judgements-acc ((judge1 pseudo-termp)
+                              (judge2 pseudo-termp)
+                              (acc pseudo-termp)
                               state)
-  :returns (judgements pseudo-termp)
-  (supertype-judgements-acc judge supertype-alst thms judge state))
-
-#|
-(defthm test (implies (integerp x) (rationalp x)))
-(supertype-judgements '(if (integerp x) 't 'nil)
-                      '((integerp . rationalp) (rationalp . nil))
-                      '((((type . integerp) (super-type . rationalp)) . test))
-                      state)
-
-(supertype-judgements '(if (maybe-rational-integer-consp
-                            (if (rational-integer-alistp al)
-                                (if (rationalp r1)
-                                    (assoc-equal r1 al)
-                                    'nil)
-                                'nil))
-                           't
-                           'nil)
-                      '((maybe-rational-integer-consp . nil) (booleanp . nil)
-                        (symbolp . nil) (maybe-integerp . nil)
-                        (rational-integer-alistp . nil))
-                      '()
-                      state
-                      )
-|#
-
-(define supertype-of?-clocked ((type1 symbolp)
-                               (type2 symbolp)
-                               (supertype-alst type-to-type-alist-p)
-                               (thms type-tuple-to-thm-alist-p)
-                               (clock natp)
-                               state)
-  :returns (ok booleanp)
-  :measure (nfix clock)
-  (b* ((type1 (symbol-fix type1))
-       (type2 (symbol-fix type2))
-       (clock (nfix clock))
-       ((if (zp clock))
-        (er hard? 'type-inference=>supertype-of?-clocked
-            "Run out of clock.~%"))
-       ((if (equal type1 type2)) t)
-       (conspair (assoc-equal type2 supertype-alst))
-       ((unless conspair)
-        (er hard? 'type-inference=>supertype-of?
-            "Can't find ~p0 in type-to-supertype-alist.~%" type1))
-       (supertype (cdr conspair))
-       ((unless supertype) nil)
-       ((unless (look-up-type-tuple-to-thm-alist type2 supertype thms state))
-        nil))
-    (supertype-of?-clocked type1 supertype supertype-alst thms (1- clock) state)))
-
-(define supertype-of? ((type1 symbolp)
-                       (type2 symbolp)
-                       (supertype-alst type-to-type-alist-p)
-                       (thms type-tuple-to-thm-alist-p)
-                       state)
-  :returns (ok booleanp)
-  (supertype-of?-clocked type1 type2 supertype-alst thms
-                         (len supertype-alst) state))
-
-(define judgements-upper-bound ((judge1 pseudo-termp)
-                                (judge2 pseudo-termp)
-                                (supertype-alst type-to-type-alist-p)
-                                (thms type-tuple-to-thm-alist-p)
-                                state)
-  :returns (upper-bound pseudo-termp)
-  (b* ((judge1 (pseudo-term-fix judge1))
-       (judge2 (pseudo-term-fix judge2))
-       ((unless (and (type-predicate-p judge1 supertype-alst)
-                     (type-predicate-p judge2 supertype-alst)))
-        (er hard? 'type-inference=>judgements-upper-bound
-            "~p0 or ~p1 are not type-predicate(s).~%" judge1 judge2))
-       ((list* type1 term1) judge1)
-       ((list* type2 term2) judge2)
-       ((unless (equal term1 term2))
-        (er hard? 'type-inference=>supertype-of?
-            "Predicate ~p0 and ~p1 are for difference terms.~%"
-            judge1 judge2))
-       (judge1>=judge2? (supertype-of? type1 type2 supertype-alst thms state))
-       ((if judge1>=judge2?) judge1)
-       (judge2>=judge1? (supertype-of? type2 type1 supertype-alst thms state))
-       ((if judge2>=judge1?) judge2))
-    nil))
-
-(define union-judgements-12lst ((judge pseudo-termp)
-                                (judge-conj pseudo-termp)
-                                (supertype-alst type-to-type-alist-p)
-                                (thms type-tuple-to-thm-alist-p)
-                                (acc pseudo-termp)
-                                state)
-  :measure (acl2-count (pseudo-term-fix judge-conj))
   :returns (union pseudo-termp)
-  (b* ((judge (pseudo-term-fix judge))
-       (judge-conj (pseudo-term-fix judge-conj))
-       (acc (pseudo-term-fix acc))
-       ((unless (is-conjunct? judge-conj))
-        (er hard? 'type-inference=>union-judgements-12lst
-            "~p0 is not a conjunction.~%" judge-conj))
-       ((if (equal judge-conj ''t)) acc)
-       ((list* & cond then &) judge-conj)
-       (upper-bound
-        (judgements-upper-bound judge cond supertype-alst thms state))
-       ((unless upper-bound)
-        (union-judgements-12lst judge then supertype-alst thms acc state))
-       ((if (path-test acc upper-bound state))
-        (union-judgements-12lst judge then supertype-alst thms acc state)))
-    (union-judgements-12lst judge then supertype-alst thms
-                            `(if ,upper-bound ,acc 'nil) state)))
-
-(define union-judgements-lst2lst ((judge1 pseudo-termp)
-                                  (judge2 pseudo-termp)
-                                  (supertype-alst type-to-type-alist-p)
-                                  (thms type-tuple-to-thm-alist-p)
-                                  (acc pseudo-termp)
-                                  state)
-  :returns (union
-            pseudo-termp
-            :hints (("Goal" :in-theory (disable symbol-listp))))
-  :measure (acl2-count (pseudo-term-fix judge1))
+  :verify-guards nil
+  :measure (acl2-count (pseudo-term-fix judge2))
   (b* ((judge1 (pseudo-term-fix judge1))
        (judge2 (pseudo-term-fix judge2))
        (acc (pseudo-term-fix acc))
-       (thms (type-tuple-to-thm-alist-fix thms))
-       ((unless (is-conjunct? judge1))
-        (er hard? 'type-inference=>union-judgements
-            "~p0 is not a conjunction.~%" judge1))
-       ((if (equal judge1 ''t)) acc)
-       ((list* & cond then &) judge1)
-       (hd-acc (union-judgements-12lst cond judge2 supertype-alst thms acc state)))
-    (union-judgements-lst2lst then judge2 supertype-alst thms hd-acc state)))
+       ((if (path-test judge1 judge2 state))
+        `(if ,judge2 ,acc 'nil))
+       ((unless (is-conjunct? judge2)) acc)
+       ((if (equal judge2 ''t)) acc)
+       ((list & judge-hd judge-tl &) judge2)
+       (acc-hd (union-judgements-acc judge1 judge-hd acc state)))
+    (union-judgements-acc judge1 judge-tl acc-hd state)))
 
-;; Assumes judge1 and judge2 are type judgements over the same term
+(verify-guards union-judgements-acc)
+
 (define union-judgements ((judge1 pseudo-termp)
                           (judge2 pseudo-termp)
-                          (supertype-alst type-to-type-alist-p)
-                          (thms type-tuple-to-thm-alist-p)
                           state)
   :returns (union pseudo-termp)
-  (union-judgements-lst2lst judge1 judge2 supertype-alst thms ''t state))
+  (union-judgements-acc judge1 judge2 ''t state))
 
 #|
 (defthm test (implies (integerp x) (rationalp x)))
 (union-judgements '(if (rationalp x) (if (integerp x) 't 'nil) 'nil)
                   '(if (rationalp x) (if (integerp x) 't 'nil) 'nil)
-                  '((integerp . rationalp) (rationalp . nil))
-                  '((((type . integerp) (super-type . rationalp)) . test))
                   state)
 
-(union-judgements '(if (maybe-rational-integer-consp (if (rationalp r1)
-                                                         (assoc-equal r1 al)
-                                                         'nil))
-                       't
-                       'nil)
-                  '(if
-                  (booleanp (if (rationalp r1)
-                                (assoc-equal r1 al)
-                                'nil))
-                  (if
-                   (symbolp (if (rationalp r1)
-                                (assoc-equal r1 al)
-                                'nil))
-                   (if
-                     (maybe-rational-integer-consp (if (rationalp r1)
-                                                       (assoc-equal r1 al)
-                                                       'nil))
-                     (if (maybe-integerp (if (rationalp r1)
-                                             (assoc-equal r1 al)
-                                             'nil))
-                         (if (rational-integer-alistp (if (rationalp r1)
-                                                          (assoc-equal r1 al)
-                                                          'nil))
-                             't
-                             'nil)
-                         'nil)
-                     'nil)
-                   'nil)
-                  'nil)
-                  '((maybe-rational-integer-consp . nil) (booleanp . nil)
-                    (symbolp . nil) (maybe-integerp . nil)
-                    (rational-integer-alistp . nil))
-                  '()
+(union-judgements '(if (rationalp x) 't 'nil)
+                  '(if (rationalp x) (if (integerp x) 't 'nil) 'nil)
                   state)
 |#
 
@@ -1087,84 +739,245 @@
   :hints (("Goal"
            :in-theory (disable pseudo-termp))))
 
-(encapsulate ()
-  (local
-   (in-theory (disable (:definition assoc-equal)
-                       (:definition symbol-listp)
-                       (:rewrite is-conjunct?-very-stupid)
-                       (:rewrite lambda-of-pseudo-lambdap)
-                       (:rewrite consp-of-pseudo-lambdap)
-                       (:rewrite pseudo-term-listp-of-symbol-listp)
-                       (:rewrite consp-of-cdr-of-pseudo-lambdap))))
+(defines super/subtype-transitive-closure
+  :well-founded-relation l<
+  :verify-guards nil
 
-(define subtype-judgement-single ((judgement pseudo-termp)
-                                  (path-cond pseudo-termp)
-                                  (options type-options-p)
-                                  state)
-  :returns (new-judgement
-            pseudo-termp
-            :hints (("Goal"
-                     :in-theory
-                     (disable (:definition pseudo-termp)
-                              (:rewrite
-                               consp-of-pseudo-lambdap)
-                              (:rewrite
-                               acl2::pseudo-lambdap-of-car-when-pseudo-lambda-listp)
-                              (:rewrite pseudo-term-listp-of-symbol-listp)
-                              (:rewrite
-                               acl2::symbol-listp-of-cdr-when-symbol-listp)
-                              (:rewrite default-cdr)
-                              (:rewrite acl2::pseudo-termp-opener)
-                              (:rewrite equal-fixed-and-x-of-pseudo-termp)))))
-  :ignore-ok t ;; for var
-  (b* ((options (type-options-fix options))
-       (judgement (pseudo-term-fix judgement))
-       ((unless (type-predicate-p judgement (type-options->supertype options)))
-        (er hard? 'type-inference=>subtype-judgement-single
-            "Judgement to be strengthened ~p0 is malformed.~%" judgement))
-       (option-description (type-options->option options))
-       ((list type term) judgement)
-       (maybe-type? (is-maybe-type? type option-description))
-       ((unless maybe-type?) judgement)
-       (not-nil?
-        (path-test path-cond term state))
-       ((unless not-nil?) judgement)
-       (nonnil-name
-        (get-nonnil-thm type option-description))
-       (nonnil-thm
-        (acl2::meta-extract-formula-w nonnil-name (w state)))
-       ((unless (pseudo-termp nonnil-thm))
-        (er hard? 'type-inference=>subtype-judgement-single
+  (define super/subtype ((type symbolp)
+                         (type-alst type-to-types-alist-p)
+                         (closure symbol-listp)
+                         (clock natp)) ;; clock is the length of the supertype-alst
+    :measure (list (nfix clock) (acl2-count (symbol-fix type)))
+    :returns (closure symbol-listp)
+    (b* ((type (symbol-fix type))
+         (type-alst (type-to-types-alist-fix type-alst))
+         (closure (symbol-list-fix closure))
+         (clock (nfix clock))
+         ((if (zp clock)) closure)
+         (exist? (member-equal type closure))
+         ((if exist?) closure)
+         (new-closure (cons type closure))
+         (item (assoc-equal type type-alst))
+         ((unless item)
+          (er hard? 'type-inference=>super/subtype
+              "Type ~p0 doesn't exist in the supertype alist.~%" type))
+         ((unless (cdr item)) new-closure)
+         (type-lst (cdr item)))
+      (super/subtype-list type-lst type-alst new-closure (1- clock))))
+
+  (define super/subtype-list ((type-lst symbol-listp)
+                              (type-alst type-to-types-alist-p)
+                              (closure symbol-listp)
+                              (clock natp))
+    :measure (list (nfix clock) (acl2-count (symbol-list-fix type-lst)))
+    :returns (closure symbol-listp)
+    (b* ((type-lst (symbol-list-fix type-lst))
+         (type-alst (type-to-types-alist-fix type-alst))
+         (closure (symbol-list-fix closure))
+         (clock (nfix clock))
+         ((unless (consp type-lst)) closure)
+         ((cons type-hd type-tl) type-lst)
+         (new-closure (super/subtype type-hd type-alst closure clock)))
+      (super/subtype-list type-tl type-alst new-closure clock)))
+  )
+
+(verify-guards super/subtype)
+
+#|
+(super/subtype 'integerp '((integerp . (rationalp maybe-integerp))
+                           (maybe-integerp . (maybe-rationalp))
+                           (rationalp . (maybe-rationalp))
+                           (maybe-rationalp . nil))
+               nil 4)
+
+(super/subtype 'rationalp '((integerp . (rationalp maybe-integerp))
+                           (maybe-integerp . (maybe-rationalp))
+                           (rationalp . (maybe-rationalp))
+                           (maybe-rationalp . nil))
+               nil 4)
+|#
+
+(local
+ (defthm pseudo-termp-of-cadr-of-consp
+   (implies (and (pseudo-termp x)
+                 (not (equal (car x) 'quote))
+                 (consp x)
+                 (consp (cdr x)))
+            (pseudo-termp (cadr x)))
+   :hints (("Goal" :in-theory (enable pseudo-termp)))))
+
+(define look-up-type-tuple-to-thm-alist ((root-type symbolp)
+                                         (type symbolp)
+                                         (thms type-tuple-to-thm-alist-p)
+                                         (term pseudo-termp)
+                                         (path-cond pseudo-termp)
+                                         state)
+  :returns (ok booleanp)
+  :guard-hints (("Goal"
+                 :in-theory (disable assoc-equal
+                                     symbol-listp
+                                     is-conjunct?-very-stupid
+                                     pseudo-term-listp-of-cdr-of-pseudo-termp
+                                     default-cdr
+                                     consp-of-pseudo-lambdap)))
+  :ignore-ok t
+  (b* ((thms (type-tuple-to-thm-alist-fix thms))
+       (path-cond (pseudo-term-fix path-cond))
+       (term (pseudo-term-fix term))
+       (tuple (make-type-tuple :type root-type
+                               :neighbour-type type))
+       (conspair (assoc-equal tuple thms))
+       ((unless conspair) nil)
+       (thm-name (cdr conspair))
+       (type-thm
+        (acl2::meta-extract-formula-w thm-name (w state)))
+       ((unless (pseudo-termp type-thm))
+        (er hard? 'type-inference=>look-up-type-tuple-to-thm-alist
             "Formula returned by meta-extract ~p0 is not a pseudo-termp: ~p1~%"
-            nonnil-name nonnil-thm))
-       ((mv ok strengthened-type)
-        (case-match nonnil-thm
-          (('implies ('if (!type var) ('not ('null var)) ''nil)
-                     (strengthened-type var))
-           (mv t strengthened-type))
-          (& (mv nil nil))))
-       ((unless (and ok (symbolp strengthened-type)))
-        (er hard? 'type-inference=>subtype-judgement-single
-            "The non-nil theorem for type ~p0 is of the wrong syntactic form ~
-              ~p1~%" type nonnil-thm)))
-    `(,strengthened-type ,term)))
+            thm-name type-thm))
+       (ok (case-match type-thm
+             (('implies (!root-type var) (!type var)) t)
+             (('implies type-predicates (!type var))
+              (and (not (equal type 'quote))
+                   (path-test type-predicates `(,root-type ,var) state)
+                   (path-test-list (term-substitution path-cond term var t)
+                                   type-predicates state)))
+             (& nil))))
+    ok))
+
+(encapsulate ()
+  (local (in-theory (disable (:definition pseudo-termp)
+                             (:rewrite lambda-of-pseudo-lambdap))))
+  (local
+   (defthm assoc-equal-of-type-tuple-to-thm-alist-p
+     (implies (and (type-tuple-to-thm-alist-p x)
+                   (assoc-equal y x))
+              (and (consp (assoc-equal y x))
+                   (symbolp (cdr (assoc-equal y x)))))))
+
+(define super/subtype-to-judgements ((root-type symbolp)
+                                     (types symbol-listp)
+                                     (term pseudo-termp)
+                                     (thms type-tuple-to-thm-alist-p)
+                                     (path-cond pseudo-termp)
+                                     (acc pseudo-termp)
+                                     state)
+  :returns (judgements pseudo-termp)
+  :measure (len types)
+  (b* ((root-type (symbol-fix root-type))
+       (types (symbol-list-fix types))
+       (term (pseudo-term-fix term))
+       (thms (type-tuple-to-thm-alist-fix thms))
+       (acc (pseudo-term-fix acc))
+       ((unless (consp types)) acc)
+       ((cons types-hd types-tl) types)
+       ((if (equal root-type types-hd))
+        (super/subtype-to-judgements root-type types-tl term thms path-cond acc
+                                     state))
+       ((unless (look-up-type-tuple-to-thm-alist root-type types-hd thms
+                                                 term path-cond state))
+        acc)
+       (type-term `(,types-hd ,term))
+       ((if (path-test acc type-term state))
+        (super/subtype-to-judgements root-type types-tl term thms path-cond acc
+                                     state)))
+    (super/subtype-to-judgements root-type types-tl term thms path-cond
+                                 `(if ,type-term ,acc 'nil) state)))
 )
 
-(define subtype-judgements ((judgements pseudo-termp)
-                            (path-cond pseudo-termp)
-                            (options type-options-p)
-                            state)
-  :returns (new-judgements pseudo-termp)
-  :measure (acl2-count (pseudo-term-fix judgements))
-  (b* ((judgements (pseudo-term-fix judgements))
-       ((unless (is-conjunct? judgements))
-        (er hard? 'type-inference=>subtype-judgements
-            "~p0 is not a conjunction.~%" judgements))
-       ((if (equal judgements ''t)) judgements)
-       ((list* & judge-hd judge-tl &) judgements))
-    `(if ,(subtype-judgement-single judge-hd path-cond options state)
-         ,(subtype-judgements judge-tl path-cond options state)
-       'nil)))
+(define super/subtype-judgement-single ((type-judgement pseudo-termp)
+                                        (path-cond pseudo-termp)
+                                        (type-alst type-to-types-alist-p)
+                                        (thms type-tuple-to-thm-alist-p)
+                                        (acc pseudo-termp)
+                                        state)
+  :guard (type-predicate-p type-judgement type-alst)
+  :returns (judgements pseudo-termp)
+  (b* ((type-judgement (pseudo-term-fix type-judgement))
+       (type-alst (type-to-types-alist-fix type-alst))
+       (acc (pseudo-term-fix acc))
+       ((unless (mbt (type-predicate-p type-judgement type-alst))) acc)
+       ((list root-type term) type-judgement)
+       (clock (len type-alst))
+       (super/subtypes
+        (super/subtype root-type type-alst nil clock)))
+    (super/subtype-to-judgements root-type super/subtypes term thms path-cond
+                                 acc state)))
+
+(define super/subtype-judgements-acc ((judge pseudo-termp)
+                                      (path-cond pseudo-termp)
+                                      (type-alst type-to-types-alist-p)
+                                      (thms type-tuple-to-thm-alist-p)
+                                      (acc pseudo-termp)
+                                      state)
+  :returns (judgements pseudo-termp)
+  :measure (acl2-count (pseudo-term-fix judge))
+  :verify-guards nil
+  (b* ((judge (pseudo-term-fix judge))
+       (acc (pseudo-term-fix acc))
+       ((if (type-predicate-p judge type-alst))
+        (super/subtype-judgement-single judge path-cond type-alst thms acc state))
+       ((unless (is-conjunct? judge)) acc)
+       ((if (equal judge ''t)) acc)
+       ((list* & cond then &) judge)
+       (first-acc (super/subtype-judgements-acc cond path-cond type-alst thms
+                                                acc state)))
+    (super/subtype-judgements-acc then path-cond type-alst thms first-acc
+                                  state)))
+
+(verify-guards super/subtype-judgements-acc)
+
+(define super/subtype-judgements-fn ((judge pseudo-termp)
+                                     (path-cond pseudo-termp)
+                                     (type-alst type-to-types-alist-p)
+                                     (thms type-tuple-to-thm-alist-p)
+                                     state)
+  :returns (judgements pseudo-termp)
+  (super/subtype-judgements-acc judge path-cond type-alst thms judge state))
+
+;; #|
+(defthm test (implies (integerp x) (rationalp x)))
+(super/subtype-judgements-fn '(if (integerp x) 't 'nil) ''t
+                             '((integerp . (rationalp)) (rationalp . nil))
+                             '((((type . integerp) (neighbour-type . rationalp)) .
+                                test))
+                             state)
+;; |#
+
+(defmacro super/subtype-judgements (judgements path-cond options state
+                                               &key which)
+  `(if (equal ,which :super)
+       (super/subtype-judgements-fn ,judgements ,path-cond
+                                    (type-options->supertype ,options)
+                                    (type-options->supertype-thm ,options)
+                                    ,state)
+     (super/subtype-judgements-fn ,judgements ,path-cond
+                                  (type-options->subtype ,options)
+                                  (type-options->subtype-thm ,options)
+                                  ,state)))
+
+;; #|
+(defthm test (implies (integerp x) (rationalp x)))
+(super/subtype-judgements '(if (integerp x) 't 'nil) ''t
+                          '((supertype (integerp rationalp)
+                                       (rationalp))
+                            (supertype-thm (((type . integerp)
+                                             (neighbour-type . rationalp))
+                                            . test))
+                            (subtype)
+                            (subtype-thm)
+                            (functions)
+                            (consp)
+                            (basic)
+                            (list)
+                            (alist)
+                            (prod)
+                            (option)
+                            (sum)
+                            (abstract))
+                          state
+                          :which :super)
+;; |#
 
 ;; extend-judgements first calcualte the subtypes then it calculate the
 ;; supertypes based on the subtypes
@@ -1173,13 +986,9 @@
                            (options type-options-p)
                            state)
   :returns (new-judgements pseudo-termp)
-  (b* ((judgements (pseudo-term-fix judgements))
-       (path-cond (pseudo-term-fix path-cond))
-       (options (type-options-fix options))
-       (supertype-alst (type-options->supertype options))
-       (supertype-thm-alst (type-options->supertype-thm options)))
-    (supertype-judgements (subtype-judgements judgements path-cond options state)
-                          supertype-alst supertype-thm-alst state)))
+  (super/subtype-judgements
+   (super/subtype-judgements judgements path-cond options state :which :sub)
+   path-cond options state :which :super))
 
 ;; reduce not's in term
 (define simple-transformer ((term pseudo-termp))
@@ -1402,11 +1211,7 @@
          (judge-else-top (type-judgement-top judge-else))
          (judge-from-then (term-substitution judge-then-top then term t))
          (judge-from-else (term-substitution judge-else-top else term t))
-         (supertype-alst (type-options->supertype options))
-         (supertype-thm-alst (type-options->supertype-thm options))
-         (judge-if-top (union-judgements judge-from-then judge-from-else
-                                         supertype-alst supertype-thm-alst
-                                         state))
+         (judge-if-top (union-judgements judge-from-then judge-from-else state))
          (judge-if-top-extended
           (extend-judgements judge-if-top path-cond options state)))
       `(if ,judge-if-top-extended
@@ -1516,24 +1321,23 @@
   :pred maybe-rational-integer-consp)
 
 (defun supertype ()
-  `((integerp . rationalp)
-    (integerp . maybe-integerp)
+  `((integerp . (rationalp maybe-integerp))
     (rationalp . nil)
     (symbolp . nil)
     (booleanp . nil)
-    (rational-integer-cons-p . maybe-rational-integer-consp)
+    (rational-integer-cons-p . (maybe-rational-integer-consp))
     (rational-integer-alistp . nil)
     (maybe-integerp . nil)
     (maybe-rational-integer-consp . nil)
     ))
 
 (defun subtype ()
-  `((rationalp . integerp)
-    (maybe-integerp . integerp)
+  `((rationalp . (integerp))
+    (maybe-integerp . (integerp))
     (integerp . nil)
     (symbolp . nil)
     (booleanp . nil)
-    (maybe-rational-integer-consp . rational-integer-cons-p)
+    (maybe-rational-integer-consp . (rational-integer-cons-p))
     (rational-integer-alistp . nil)
     (rational-integer-cons-p . nil)
     ))
@@ -1557,13 +1361,11 @@
                        rational-integer-cons-p-implies-maybe-rational-integer-consp)))
 
 (defthm maybe-integerp-can-be-integerp
-  (implies (and (maybe-integerp x)
-                (not (null x)))
+  (implies (and (maybe-integerp x) x)
            (integerp x)))
 
 (defthm maybe-rational-integer-consp-can-be-rational-integer-cons-p
-  (implies (and (maybe-rational-integer-consp x)
-                (not (null x)))
+  (implies (and (maybe-rational-integer-consp x) x)
            (rational-integer-cons-p x)))
 
 (defun subtype-thm ()
@@ -1684,9 +1486,6 @@
                                                             :cdr-type 'integerp
                                                             :cdr-thm nil))))
 
-(defthm nil-thm-rational-integer-alistp
-  (rational-integer-alistp nil))
-
 (defun alist ()
   `((rational-integer-alistp . ,(make-alist-type-description :recognizer 'rational-integer-alistp
                                                              :fixer 'rational-integer-alist-fix
@@ -1696,22 +1495,6 @@
                                                              :assoc-equal-thm nil
                                                              ))))
 
-(defthm nil-thm-maybe-rational-integer-consp
-  (maybe-rational-integer-consp nil))
-
-(defthm non-nil-thm-maybe-rational-integer-consp
-  (implies (and (maybe-rational-integer-consp x)
-                (not (null x)))
-           (rational-integer-cons-p x)))
-
-(defthm nil-thm-maybe-integerp
-  (maybe-integerp nil))
-
-(defthm non-nil-thm-maybe-integerp
-  (implies (and (maybe-integerp x)
-                (not (null x)))
-           (integerp x)))
-
 (defun option ()
   `((maybe-integerp . ,(make-option-type-description :recognizer
                                                      'maybe-integerp
@@ -1720,7 +1503,6 @@
                                                      :some-constructor-thm nil
                                                      :none-constructor-thm nil
                                                      :some-destructor-thm nil
-                                                     :non-nil-thm 'non-nil-thm-maybe-integerp
                                                      ))
     (maybe-rational-integer-consp . ,(make-option-type-description :recognizer 'maybe-rational-integer-consp
                                                                    :fixer 'maybe-rational-integer-cons-fix
@@ -1728,9 +1510,8 @@
                                                                    'rational-integer-cons-p
                                                                    :some-constructor-thm nil
                                                                    :none-constructor-thm nil
-                                                                   :some-destructor-thm nil
-                                                                   :non-nil-thm 'non-nil-thm-maybe-rational-integer-consp
-                                                                   ))))
+                                                                   :some-destructor-thm
+                                                                   nil))))
 
 (defun options ()
   (b* ((supertype (supertype))
